theories/Strings/PString.v
@@ -12,6 +12,10 @@ Require Import ZArith.
 #[local] Open Scope list_scope.
 #[local] Arguments to_Z _/ : simpl nomatch.
 
+#[local] Instance Op_max_length : ZifyClasses.CstOp max_length :=
+  { TCst := 16777211%Z ; TCstInj := eq_refl }.
+Add Zify CstOp Op_max_length.
+
 #[local] Ltac case_if :=
   lazymatch goal with
   | |- context C [if ?b then _ else _] => destruct b eqn:?
@@ -219,12 +223,51 @@ Qed.
 
 (** * Properties of string comparison *)
 
-
 Lemma char63_compare_refl (c1 c2 : char63) :
   char63_compare c1 c2 = Eq <-> c1 = c2.
 Proof.
   rewrite Uint63.compare_spec, Z.compare_eq_iff.
   split; [apply to_Z_inj|intros <-; reflexivity].
+Qed.
+
+Lemma char63_compare_antisym (c1 c2 : char63) :
+  char63_compare c2 c1 = CompOpp (char63_compare c1 c2).
+Proof.
+  rewrite !Uint63.compare_spec. apply Z.compare_antisym.
+Qed.
+
+Lemma char63_compare_trans (c1 c2 c3 : char63) (c : comparison) :
+  char63_compare c1 c2 = c -> char63_compare c2 c3 = c -> char63_compare c1 c3 = c.
+Proof.
+  destruct c.
+  - rewrite !char63_compare_refl. intros -> ->. reflexivity.
+  - rewrite !Uint63.compare_spec. apply Zcompare_Lt_trans.
+  - rewrite !Uint63.compare_spec. apply Zcompare_Gt_trans.
+Qed.
+
+Lemma compare_refl (s : string) : compare s s = Eq.
+Proof.
+  rewrite PrimStringAxioms.compare_spec.
+  apply (List.list_compare_refl _ char63_compare_refl). reflexivity.
+Qed.
+
+Lemma compare_antisym (s1 s2 : string) :
+  compare s2 s1 = CompOpp (compare s1 s2).
+Proof.
+  rewrite !PrimStringAxioms.compare_spec.
+  apply List.list_compare_antisym.
+  - apply char63_compare_refl.
+  - apply char63_compare_antisym.
+Qed.
+
+Lemma compare_trans (c : comparison) (s1 s2 s3 : string) :
+  compare s1 s2 = c -> compare s2 s3 = c -> compare s1 s3 = c.
+Proof.
+  rewrite !PrimStringAxioms.compare_spec.
+  apply List.list_compare_trans.
+  - apply char63_compare_refl.
+  - apply char63_compare_trans.
+  - apply char63_compare_antisym.
 Qed.
 
 Lemma compare_eq_correct (s1 s2 : string) :
@@ -236,7 +279,7 @@ Qed.
 
 Lemma string_eq_ext (s1 s2 : string) :
   (length s1 = length s2 /\
-     forall i, to_Z i < to_Z (length s1) -> get s1 i = get s2 i) ->
+   forall i, to_Z i < to_Z (length s1) -> get s1 i = get s2 i) ->
   s1 = s2.
 Proof.
   intros [Hlen Hget]. apply to_list_inj.
@@ -247,6 +290,19 @@ Proof.
     { rewrite of_Z_spec, Z.mod_small, Nat2Z.id; lia. }
     rewrite <-!get_spec. apply Hget.
     rewrite of_Z_spec, Z.mod_small; lia.
+Qed.
+
+Lemma to_list_firstn_skipn_middle (s : string) (i : int) :
+  to_Z i < to_Z (length s) ->
+  to_list s = List.firstn (to_nat i) (to_list s) ++
+                get s i :: List.skipn (to_nat (i + 1)) (to_list s).
+Proof.
+  intros Hi.
+  assert (to_nat (i + 1) = S (to_nat i)) as ->.
+  { rewrite add_spec, Z.mod_small, Z2Nat.inj_add; lia. }
+  symmetry. apply List.firstn_skipn_middle.
+  rewrite get_spec. apply List.nth_error_nth'.
+  rewrite <-length_spec. lia.
 Qed.
 
 Lemma compare_spec (s1 s2 : string) (c : comparison) :
@@ -266,109 +322,110 @@ Lemma compare_spec (s1 s2 : string) (c : comparison) :
         end
     end.
 Proof.
-  rewrite compare_spec, (List.list_compare_prefix_spec _ char63_compare_refl).
-  split.
-  - intros (prefix & xs' & ys' & H1 & H2 & H).
-    exists (of_Z (Z.of_nat (List.length prefix))).
-    assert (Z.of_nat (Datatypes.length prefix) <= to_Z max_length) as Hltmax.
-    { transitivity (Z.of_nat (List.length (to_list s1))).
-      - rewrite H1, List.length_app. simpl. lia.
-      - pose proof to_list_length s1; lia. }
-    simpl in Hltmax.
-    rewrite !length_spec_Z, H1, H2, !List.length_app.
-    rewrite of_Z_spec, Z.mod_small; [|lia].
-    repeat split.
-    + lia.
-    + lia.
-    + intros j Hj. rewrite !get_spec.
-      rewrite H1, H2, !List.app_nth1; [reflexivity | lia | lia].
-    + pose proof length_spec s1 as Hlen1.
-      pose proof length_spec s2 as Hlen2.
-      rewrite !length_spec_int, H1, H2, !List.length_app, !eqb_eq.
-      rewrite H1, List.length_app in Hlen1.
-      rewrite H2, List.length_app in Hlen2.
-      rewrite !of_Z_spec, !Z.mod_small; try (rewrite <-?Hlen1, <-?Hlen2; lia).
-      destruct xs' as [|x xs']; simpl; case_if; try lia.
-      { destruct ys' as [|y ys']; simpl.
-        - rewrite Nat.add_0_r, Z.eqb_refl. assumption.
-        - case_if; [exfalso; lia | assumption]. }
-      destruct ys' as [|y ys']; simpl; case_if; try lia; try assumption.
-      rewrite !get_spec, H1, H2.
-      rewrite !of_Z_spec, !Z.mod_small, Nat2Z.id; [|lia].
-      rewrite !List.nth_middle. assumption.
+  rewrite compare_spec. split.
+  - pose proof List.list_compareP _ char63_compare_refl (to_list s1) (to_list s2) as Hcmp.
+    revert Hcmp. remember (List.list_compare _ _ _) as c' eqn:Hc'. intros Hcmp Hcc'.
+    induction Hcmp as [H|y ys H|x xs H|????? H1 H2 H|????? H1 H2 H]; clear Hc'; subst c.
+    + apply to_list_inj in H. subst s2. exists (length s1).
+      rewrite eqb_eq, Z.eqb_refl. repeat split; lia.
+    + exists (length s1).
+      rewrite !eqb_eq, Z.eqb_refl, !length_spec_Z, H, List.length_app.
+      repeat split; [lia|lia| |].
+      * intros j Hj. rewrite !get_spec, H. rewrite List.app_nth1; [reflexivity|lia].
+      * simpl in *. case_if; [exfalso; lia|reflexivity].
+    + exists (length s2).
+      rewrite !eqb_eq, Z.eqb_refl, !length_spec_Z, H, List.length_app.
+      repeat split; [lia|lia| |].
+      * intros j Hj. rewrite !get_spec, H. rewrite List.app_nth1; [reflexivity|lia].
+      * simpl in *. case_if; [exfalso; lia|reflexivity].
+    + exists (of_nat (List.length prefix)).
+      assert (Z.of_nat (List.length prefix) < wB) as Hprefix.
+      { pose proof f_equal (@List.length _) H1 as Hlen.
+        pose proof valid_length s1 as Hmax.
+        rewrite <-length_spec, List.length_app in Hlen. lia. }
+      rewrite !eqb_eq, !length_spec_Z, H1, H2, !List.length_app.
+      rewrite of_Z_spec, Z.mod_small; [|lia].
+      repeat split; [lia|lia| |].
+      * intros i Hj. rewrite !get_spec, H1, H2, !List.app_nth1; [reflexivity|lia|lia].
+      * simpl in *; repeat case_if; try lia.
+        rewrite !get_spec, H1, H2.
+        do 2 (rewrite List.app_nth2; [|rewrite of_Z_spec, Z.mod_small; lia]).
+        rewrite !of_Z_spec, Z.mod_small, Nat2Z.id, Nat.sub_diag; [|lia].
+        simpl. rewrite H. reflexivity.
+    + exists (of_nat (List.length prefix)).
+      assert (Z.of_nat (List.length prefix) < wB) as Hprefix.
+      { pose proof f_equal (@List.length _) H1 as Hlen.
+        pose proof valid_length s1 as Hmax.
+        rewrite <-length_spec, List.length_app in Hlen. lia. }
+      rewrite !eqb_eq, !length_spec_Z, H1, H2, !List.length_app.
+      rewrite of_Z_spec, Z.mod_small; [|lia].
+      repeat split; [lia|lia| |].
+      * intros i Hj. rewrite !get_spec, H1, H2, !List.app_nth1; [reflexivity|lia|lia].
+      * simpl in *; repeat case_if; try lia.
+        rewrite !get_spec, H1, H2.
+        do 2 (rewrite List.app_nth2; [|rewrite of_Z_spec, Z.mod_small; lia]).
+        rewrite !of_Z_spec, Z.mod_small, Nat2Z.id, Nat.sub_diag; [|lia].
+        simpl. rewrite H. reflexivity.
   - intros (i & Hs1 & Hs2 & Hget & H).
-    exists (List.firstn (to_nat i) (to_list s1)).
-    exists (List.skipn (to_nat i) (to_list s1)).
-    exists (List.skipn (to_nat i) (to_list s2)).
-    assert (List.firstn (to_nat i) (to_list s1) = List.firstn (to_nat i) (to_list s2)) as Heq.
-    { apply (List.nth_ext _ _ 0%uint63 0%uint63).
-      - rewrite !List.length_firstn. rewrite !Nat.min_l; [reflexivity| |].
-        all: rewrite <-length_spec; lia.
-      - rewrite List.length_firstn, Nat.min_l.
-        2: rewrite <-length_spec; lia.
-        intros n Hn.
-        assert ((of_Z (Z.of_nat n) <? i)%uint63 = true) as Hi.
-        { apply ltb_spec. rewrite of_Z_spec, Z.mod_small; lia. }
-        pose proof Hget (of_Z (Z.of_nat n)) ltac:(lia) as Hget.
-        rewrite !get_spec in Hget.
-        rewrite of_Z_spec, Z.mod_small, Nat2Z.id in Hget; [|lia].
-        rewrite !List.nth_firstn. repeat case_if; lia. }
-    rewrite Heq at 2. rewrite !List.firstn_skipn. repeat split.
-    destruct (i =? length s1)%uint63 eqn:His1.
-    + rewrite (List.skipn_all2 (to_list s1)).
-      2: rewrite <-length_spec; lia.
-      destruct (i =? length s2)%uint63 eqn:His2.
-      * rewrite (List.skipn_all2 (to_list s2)).
-        2: rewrite <-length_spec; lia.
-        assumption.
-      * destruct (List.skipn (to_nat i) (to_list s2)) eqn:Hskip; [|assumption].
-        exfalso. apply List.skipn_all_iff in Hskip.
-        rewrite <-length_spec in Hskip. lia.
-    + destruct (List.skipn (to_nat i) (to_list s1)) eqn:Hskip1.
-      { exfalso. apply List.skipn_all_iff in Hskip1. rewrite <-length_spec in Hskip1. lia. }
-      destruct (i =? length s2)%uint63 eqn:His2.
-      { rewrite List.skipn_all2; [assumption|]. rewrite <-length_spec. lia. }
-      destruct (List.skipn (to_nat i) (to_list s2)) eqn:Hskip2.
-      { exfalso. apply List.skipn_all_iff in Hskip2. rewrite <-length_spec in Hskip2. lia. }
-      assert (c0 = get s1 i) as ->.
-      { assert (List.nth_error (List.skipn (to_nat i) (to_list s1)) 0 = Some c0) as Hc0.
-        { rewrite Hskip1. reflexivity. }
-        rewrite List.nth_error_skipn, Nat.add_0_r in Hc0.
-        rewrite get_spec.
-        eapply List.nth_error_nth in Hc0. rewrite Hc0. reflexivity. }
-      assert (c1 = get s2 i) as ->.
-      { assert (List.nth_error (List.skipn (to_nat i) (to_list s2)) 0 = Some c1) as Hc1.
-        { rewrite Hskip2. reflexivity. }
-        rewrite List.nth_error_skipn, Nat.add_0_r in Hc1.
-        rewrite get_spec.
-        eapply List.nth_error_nth in Hc1. rewrite Hc1. reflexivity. }
-      assumption.
-Qed.
-
-Lemma compare_refl (s : string) : compare s s = Eq.
-Proof.
-  rewrite PrimStringAxioms.compare_spec.
-  apply (List.list_compare_refl _ char63_compare_refl). reflexivity.
+    pose proof valid_length s1 as Hlen1.
+    pose proof valid_length s2 as Hlen2.
+    apply (List.list_compare_spec_complete char63_compare_refl).
+    repeat case_if; subst.
+    + apply List.ListCompareEq. f_equal. apply string_eq_ext. split; [lia|].
+      intros j Hj. apply Hget. lia.
+    + assert (to_Z (length s1) < to_Z (length s2)) as Hlen by lia.
+      assert (i = length s1) by lia; subst i.
+      apply (List.ListCompareShorter _ _ (get s2 (length s1))
+               (List.skipn (to_nat (length s1 + 1)) (to_list s2))).
+      rewrite (to_list_firstn_skipn_middle s2 (length s1)) at 1; [|lia].
+      f_equal. apply (List.nth_ext _ _ 0%uint63 0%uint63).
+      { rewrite List.length_firstn, <-!length_spec. lia. }
+      rewrite List.length_firstn, <-!length_spec, Nat.min_l; [|lia].
+      intros n Hn. rewrite List.nth_firstn. case_if; [|lia].
+      pose proof Hget (of_nat n). rewrite !get_spec in H.
+      rewrite of_Z_spec, Z.mod_small, Nat2Z.id in H; [|lia].
+      symmetry. apply H. lia.
+    + assert (to_Z (length s2) < to_Z (length s1)) as Hlen by lia.
+      assert (i = length s2) by lia; subst i.
+      eapply (List.ListCompareLonger _ _ (get s1 (length s2))
+                (List.skipn (to_nat (length s2 + 1)) (to_list s1))).
+      rewrite (to_list_firstn_skipn_middle s1 (length s2)) at 1; [|lia].
+      f_equal. apply (List.nth_ext _ _ 0%uint63 0%uint63).
+      { rewrite List.length_firstn, <-!length_spec. lia. }
+      rewrite List.length_firstn, <-!length_spec, Nat.min_l; [|lia].
+      intros n Hn. rewrite List.nth_firstn. case_if; [|lia].
+      pose proof Hget (of_nat n). rewrite !get_spec in H.
+      rewrite of_Z_spec, Z.mod_small, Nat2Z.id in H; [|lia].
+      apply H. lia.
+    + enough (
+          exists p l1 l2,
+            to_list s1 = p ++ get s1 i :: l1 /\
+              to_list s2 = p ++ get s2 i :: l2
+        ) as (p & l1 & l2 & Hp1 & Hp2).
+      { revert H. destruct (_ ?= _)%uint63 eqn:Hi; [intros []|intros -> ..].
+        - eapply List.ListCompareLt; solve [eauto].
+        - eapply List.ListCompareGt; solve [eauto]. }
+      exists (to_list (sub s1 0 i)).
+      exists (to_list (sub s1 (i + 1) (length s1 - i - 1))).
+      exists (to_list (sub s2 (i + 1) (length s2 - i - 1))).
+      rewrite !sub_spec; simpl.
+      rewrite !(List.firstn_all2 (n:=to_nat (length _ - _ - _))).
+      2-3: repeat progress rewrite ?List.length_skipn, ?Uint63.add_spec,
+            ?Uint63.sub_spec, ?Z.mod_small, ?Z.min_r, <-?length_spec; simpl; lia.
+      split; [apply to_list_firstn_skipn_middle; lia|].
+      rewrite (to_list_firstn_skipn_middle s2 i) at 1; [|lia].
+      enough (sub s2 0 i = sub s1 0 i) as H12.
+      { f_equal. apply (f_equal to_list) in H12. revert H12.
+        rewrite !sub_spec. simpl. intros ->. reflexivity. }
+      apply string_eq_ext; split.
+      { rewrite !sub_length_spec; lia. }
+      rewrite sub_length_spec; [|lia|lia].
+      intros j Hj. rewrite !sub_get_spec; [|lia..].
+      ring_simplify (0 + j)%uint63. symmetry. apply Hget. assumption.
 Qed.
 
 Lemma compare_eq (s1 s2 : string) : compare s1 s2 = Eq <-> s1 = s2.
 Proof. split; [apply compare_eq_correct|intros []; apply compare_refl]. Qed.
-
-Lemma compare_antisym (s1 s2 : string) : compare s2 s1 = CompOpp (compare s1 s2).
-Proof.
-  pose proof (proj1 (compare_spec s1 s2 (compare s1 s2)) eq_refl) as Hcmp.
-  destruct Hcmp as (i & Hs1 & Hs2 & Hget & H).
-  rewrite compare_spec. exists i. repeat split.
-  - assumption.
-  - assumption.
-  - intros j Hj. symmetry. apply Hget. assumption.
-  - repeat case_if; try (rewrite H; reflexivity).
-    revert H. rewrite !Uint63.compare_spec, Z.compare_antisym.
-    destruct (to_Z (get s2 i) ?= to_Z (get s1 i)) eqn:Hcmp; simpl.
-    + intros Hfalse. exact Hfalse.
-    + intros ->. reflexivity.
-    + intros ->. reflexivity.
-Qed.
 
 Lemma compare_lt_spec (s1 s2 : string) :
   compare s1 s2 = Lt <->
@@ -393,37 +450,6 @@ Proof.
     destruct H as [(-> & Hi)|(Hi1 & Hi2 & H)].
     + repeat case_if; try reflexivity; lia.
     + repeat case_if; try reflexivity; try inversion H; lia.
-Qed.
-
-Lemma compare_trans (c : comparison) (s1 s2 s3 : string) :
-  compare s1 s2 = c -> compare s2 s3 = c -> compare s1 s3 = c.
-Proof.
-  rewrite !compare_spec.
-  setoid_rewrite Uint63.compare_def_spec; unfold compare_def.
-  intros [i1 (Hi1s1&Hi1s2&Hi1&H1)] [i2 (Hi2s2&Hi2s3&Hi2&H2)].
-  destruct (i1 <? i2)%uint63 eqn:Hlt; [exists i1 | exists i2]; repeat split; try lia.
-  - intros j Hji1.
-    assert ((j <? i2)%uint63 = true) as Hji2 by lia.
-    pose proof (Hi1 j Hji1) as Hj1.
-    pose proof (Hi2 j ltac:(lia)) as Hj2.
-    revert Hj1 Hj2. intros -> <-. reflexivity.
-  - clear H2; revert H1.
-    assert (get s2 i1 = get s3 i1) as Hs2s3. { apply Hi2. lia. }
-    repeat case_if; intros H1; try assumption; try lia; try subst c.
-  - intros j Hji2.
-    assert ((j <? i1)%uint63 = true) as Hji1 by lia.
-    pose proof (Hi1 j ltac:(lia)) as Hj1.
-    pose proof (Hi2 j Hji2) as Hj2.
-    revert Hj1 Hj2. intros -> <-. reflexivity.
-  - destruct (i1 =? i2)%uint63 eqn:Heqi1i2.
-    + apply eqb_spec in Heqi1i2. subst i2. revert H1 H2.
-      repeat case_if.
-      all: intros H1; try rewrite H1; try inversion H1.
-      all: intros H2; try rewrite H2; try inversion H2.
-      all: try reflexivity; lia.
-    + clear H1; revert H2.
-      assert (get s1 i2 = get s2 i2) as Hs1s2. { apply Hi1. lia. }
-      repeat case_if; intros H1; try assumption; try lia; try subst c.
 Qed.
 
 (** * Properties of make *)
